

TF approximation for unbound electrons

The density of unbound electrons in a hybrid quantum/TF model is (Rozmus 1972):

$$\rho_{ub}(r) = \frac{\sqrt{2}}{\pi^2 c^3} [T \varphi(r)]^{3/2} \left\{ I_{1/2}(z) + \frac{5}{4} \frac{\hbar^2 T}{\varphi(r)} I_{3/2}(z) \right. \\ \left. + \frac{7}{32} \frac{\hbar^2 T^2}{\varphi^2(r)} I_{5/2}(z) + G \left(\frac{T}{\varphi(r)} \right)^3 \right\},$$

where $\varphi(r) = \{ M^2 c^4 + [r' V'(r)]^2 \}^{1/2}$,

$$I_\nu(z) = \int_{-\frac{V(r)}{T}}^{\infty} \frac{t^\nu}{e^{(t-z)} + 1} dt,$$

$$V(r) = V_{en}(r) + V_{Hoc}(r),$$

$$z(r) = \frac{\mu - V(r) + M c^2 - \varphi(r)}{T}.$$

We work in the non-relativistic limit, so:

$$\hbar T \ll M c^2 \quad \& \quad |r' V'(r)| \ll M c^2$$

$$\Rightarrow \varphi(r) \approx M c^2, \quad M_e = 1 \text{ in atomic units}$$

Hence in this limit, $\rho_{ub}(r)$ is equal to:

$$\rho_{ub}(r) = \frac{\sqrt{2}}{\pi^2} T^{3/2} \int_{-V(r)/T}^{\infty} dx \frac{x^{1/2}}{e^{(x - [\mu - V(r)]/T)} + 1}$$

We make the following change of variables:
 ~~$x = y$~~

$$x = \frac{y}{T} \Rightarrow dx = \frac{dy}{T}$$

$$\Rightarrow \rho_{\text{ub}}(r) = \frac{\sqrt{2}}{\pi^2} \int_{-V(r)}^{\infty} dy \frac{y^{1/2}}{e^{(y^2 - \mu - V(r))/T} + 1}$$

This is very similar to the density of the ideal electron gas, which is a special case of the above when $V(r) = 0$.

The ~~total~~ number of unbound electrons is then given by

$$N_{\text{ub}} = \int r^2 \rho_{\text{ub}}(r) dr$$

And μ found in the usual manner by enforcing $N_{\text{ub}}(r) + N_{\text{b}}(r) = Z$.

Now we compute the energy of the unbound electrons. ~~Again~~, In the relativistic limit this is given by:

$$\begin{aligned} \rho_{\text{ub}}(r) E_{\text{ub}} &= \frac{1}{\pi^2 c^3} T^2 \int_{x_0}^{\infty} dx \frac{[T^2 x^2 + 2xTq(r)]^{1/2} [Tx + q(r)] [x - x_0(r)]}{e^{x - Z(r)} + 1} \\ &\stackrel{q(r) \gg xT}{\approx} \frac{1}{\pi^2 c^3} T^2 \int_0^{\infty} dx \frac{\sqrt{2} q^{3/2}(r) (Tx)^{1/2} [x - x_0(r)]}{e^{x - Z(r)} + 1} \\ &\stackrel{q(r) \approx mc^2}{=} \frac{\sqrt{2}}{\pi^2} T^{5/2} \int_0^{\infty} dx \frac{x^{1/2} [x - x_0(r)]}{e^{x - Z(r)} + 1} \end{aligned}$$

Making the substitution $x = y/T$ yields:

The unbound energy E_{ub} is equal to:

$$E_{ub} = 4\pi \int_0^L dr r^2 \rho_{ub}^{ub}(r)$$

Making the change of variables $x = y/T$ yields:

$$\rho_{ub}^{ub}(r) = \frac{\sqrt{2}}{\pi^2} \int_{-V(r)}^{\infty} \frac{y^{1/2} (y + V(r))}{e^{(y - \mu - V(r))/T} + 1} dy$$

$$= \frac{\sqrt{2}}{\pi^2} \left\{ \int_{-V(r)}^{\infty} \frac{y^{3/2}}{e^{(y - \mu - V(r))/T} + 1} dy \right.$$

$$\left. + V(r) \int_{-V(r)}^{\infty} \frac{y^{1/2}}{e^{(y - \mu - V(r))/T} + 1} dy \right\}$$

$$= \frac{\sqrt{2}}{\pi^2} \int_{-V(r)}^{\infty} \frac{y^{3/2}}{e^{(y - \mu - V(r))/T} + 1} dy + V(r) \rho_{ub}(r)$$

And hence:

$$E_{ub} = 4\pi \int_0^L dr r^2 \int_{-V(r)}^{\infty} \frac{\sqrt{2}}{\pi^2} \frac{y^{3/2}}{e^{(y - \mu - V(r))/T} + 1} dy + 4\pi \int_0^L dr r^2 V(r) \rho_{ub}(r)$$

Again, this reduces to the ideal expression for $V(r) = 0$.